BASE <http://www.w3.org/ns/shapetrees>
PREFIX : <#>
PREFIX rdf: <http://www.w3.org/1999/02/22-rdf-syntax-ns#>
PREFIX xsd: <http://www.w3.org/2001/XMLSchema#>
PREFIX rdfs: <http://www.w3.org/2000/01/rdf-schema#>
PREFIX dcterms: <http://purl.org/dc/terms/>
PREFIX owl: <http://www.w3.org/2002/07/owl#>

<>
  dcterms:issued "2020-07-01"^^xsd:date ;
  dcterms:modified "2020-07-06"^^xsd:date ;
  rdfs:label "ShapeTree terms"@en .

# ShapeTree Class
#############################################################################
# Defines a tree of related resources which combine to enable some task
# see: https://shapetrees.org/TR/specification/
#############################################################################
:ShapeTree
  a rdfs:Class ;
  rdfs:comment "Defines a composite data structure including a tree of resources and validation criteria"@en ;
  rdfs:isDefinedBy <> ;
  rdfs:label "Shape Tree"@en .

:expectsType
  a owl:ObjectProperty ;
  rdfs:domain :ShapeTree ;
  rdfs:range [ owl:oneOf ( :Container :Resource ) ] ;
  rdfs:comment "Describes the expected type of resource the ShapeTree will validate against."@en ;
  rdfs:isDefinedBy <> ;
  rdfs:label "Expects Type"@en .

:contains
  a owl:ObjectProperty ;
  rdfs:domain :ShapeTree ;
  rdfs:range :ShapeTree  ;
  rdfs:comment "Links a ShapeTree to another ShapeTree that is directly contained within its planted ShapeTreeContainer"@en ;
  rdfs:isDefinedBy <> ;
  rdfs:label "Contains"@en .

:references
  a owl:ObjectProperty ;
  rdfs:domain :ShapeTree ;
  rdfs:range :ShapeTreeReference ;
  rdfs:isDefinedBy <> ;
  rdfs:comment "Links a ShapeTree to a ShapeTreeReference"@en ;
  rdfs:label "References"@en .

:shape
  a owl:ObjectProperty ;
  rdfs:domain :ShapeTree ;
  rdfs:comment "Links a ShapeTree to a Shape"@en ;
  rdfs:isDefinedBy <> ;
  rdfs:label "Shape"@en .

:supports
  a owl:ObjectProperty ;
  rdfs:domain :ShapeTree ;
  rdfs:range :ShapeTree ;
  rdfs:comment "Describes a relationship wherein a ShapeTree acts as a support for another, for purposes of indexing, aggregation, etc." ;
  rdfs:isDefinedBy <> ;
  rdfs:label "Supports"@en .

# Container IRI (maps to ldp:Container)
#############################################################################
# An IRI that represents a generalized container used in a ShapeTree
#############################################################################
:Container
  rdfs:comment "Describes a generalized container within a ShapeTree ecosystem"@en ;
  rdfs:isDefinedBy <> ;
  rdfs:label "Container"@en .


# Resource IRI (maps to ldp:Resource)
#############################################################################
# An IRI that represents a generalized resource used in a ShapeTree
#############################################################################
:Resource
  rdfs:comment "Describes a generalized RDF resource (non-container) within a ShapeTree ecosystem"@en ;
  rdfs:isDefinedBy <> ;
  rdfs:label "Resource"@en .

# NonRDFResource IRI (maps to ldp:NonRDFSource)
#############################################################################
# An IRI that represents a generalized resource used in a ShapeTree
#############################################################################
:NonRDFResource
  rdfs:comment "Describes a generalized non RDF / binary content within a ShapeTree ecosystem"@en ;
  rdfs:isDefinedBy <> ;
  rdfs:label "Non-RDF Resource"@en .


# ShapeTreeReference class
#############################################################################
# A ShapeTreeReference provides the necessary context to associate instance
# data between related ShapeTrees via a ShapePath
#############################################################################
:ShapeTreeReference
  a rdfs:Class ;
  rdfs:comment "Describes how a ShapeTree references another ShapeTree via a ShapePath"@en ;
  rdfs:isDefinedBy <> ;
  rdfs:label "ShapeTreeReference"@en .

:viaShapePath
  a owl:DatatypeProperty ;
  rdfs:domain :ShapeTreeReference ;
  rdfs:range xsd:string ;
  rdfs:comment "Describes how one ShapeTree traverses its instance data to reach another ShapeTree"@en ;
  rdfs:isDefinedBy <> ;
  rdfs:label "Via ShapePath"@en .

# ShapeTreeDecoratorIndex class
#############################################################################
# A ShapeTreeDecoratorIndex details a ShapeTree in a human-readable way.
# It is primarily used for use cases where a ShapeTree must be described to
# a user for purposes of authorization.
#############################################################################
:ShapeTreeDecoratorIndex
  a rdfs:Class ;
  rdfs:comment "Provides an index of SKOS poly-hierarchies which can be used to describe a ShapeTree"@en ;
  rdfs:isDefinedBy <> ;
  rdfs:label "ShapeTreeDecoratorIndex"@en .

:hasShapeTreeDecoratorIndex
  a owl:ObjectProperty ;
  rdfs:range :ShapeTreeDecoratorIndex ;
  rdfs:isDefinedBy <> ;
  rdfs:label "Has ShapeTree Decorator Index"@en .

:hasSet
  a owl:ObjectProperty ;
  rdfs:domain :ShapeTreeDecoratorIndex ;
  rdfs:range :ShapeTreeDecoratorSet ;
  rdfs:comment "Links between a ShapeTreeDecoratorIndex and a ShapeTreeDecoratorSet"@en ;
  rdfs:isDefinedBy <> ;
  rdfs:label "Has Set"@en .

:defaultLanguage
  a owl:ObjectProperty ;
  rdfs:domain :ShapeTreeDecoratorIndex ;
  rdfs:range xsd:language ;
  rdfs:comment "Defines default language for use with shape tree decorator when none exist matching user preferences"@en ;
  rdfs:isDefinedBy <> ;
  rdfs:label "Default language"@en .


# ShapeTreeDecoratorSet class
#############################################################################
# A ShapeTreeDecoratorSet details a set of ShapeTreeDecoratorResource classes
# Primary use is grouping TreeDecoratorResource instances by a common discriminator
# such as language or intended audience
#############################################################################
:ShapeTreeDecoratorSet
  a rdfs:Class ;
  rdfs:comment "Groups a set of ShapeTreeDecoratorResource by a given discriminator"@en ;
  rdfs:isDefinedBy <> ;
  rdfs:label "ShapeTreeDecoratorSet"@en .

:hasShapeTreeDecoratorResource
  a owl:ObjectProperty ;
  rdfs:domain :ShapeTreeDecoratorSet ;
  rdfs:range :ShapeTreeDecoratorResource ;
  rdfs:comment "Links between a ShapeTreeDecoratorSet and the decorator resource itself"@en ;
  rdfs:isDefinedBy <> ;
  rdfs:label "Has Decorator Resource"@en .

:usesLanguage
  a owl:ObjectProperty ;
  rdfs:domain :ShapeTreeDecoratorSeries ;
  rdfs:range xsd:language ;
  rdfs:comment "Describes the language used by associated ShapeTreeDecoratorResource"@en ;
  rdfs:isDefinedBy <> ;
  rdfs:label "Uses language"@en .

# ShapeTreeDecoratorResource class
#############################################################################
# A ShapeTreeDecoratorResource represents a SKOS-based resource which
# is made up of multiple st:ShapeTreeDecorator nodes that describe shape trees
#############################################################################
:ShapeTreeDecoratorResource
  a rdfs:Class ;
  rdfs:comment "Represents a SKOS-based resource which is made up of multiple st:ShapeTreeDecorator nodes that describe shape trees"@en ;
  rdfs:isDefinedBy <> ;
  rdfs:label "ShapeTreeDecoratorResource"@en .

# ShapeTreeDecorator class
#############################################################################
# A ShapeTreeDecorator represents a single descriptor of a shape tree
#############################################################################
:ShapeTreeDecorator
  a rdfs:Class ;
  rdfs:comment "A ShapeTreeDecorator represents a single descriptor of a shape tree"@en ;
  rdfs:isDefinedBy <> ;
  rdfs:label "ShapeTreeDecorator"@en .

# ShapeTreeLocator class
#############################################################################
# A shape tree locator associates a managed resource with one or more
# shape trees.
#############################################################################
:ShapeTreeLocator
  a rdfs:Class ;
  rdfs:comment "Associates a managed resource with one or more shape trees."@en ;
  rdfs:isDefinedBy <> ;
  rdfs:label "Shape Tree Locator"@en .

:hasShapeTreeLocator
  a owl:ObjectProperty ;
  rdfs:range :ShapeTreeLocator ;
  rdfs:comment "Represents the association between a subject an one or more ShapeTreeLocator"@en ;
  rdfs:isDefinedBy <> ;
  rdfs:label "Has ShapeTree Locator"@en .

:location
  a owl:ObjectProperty ;
  rdfs:range :ShapeTreeLocation ;
  rdfs:comment "Links to a ShapeTreeLocation associated with the ShapeTreeLocator"@en ;
  rdfs:isDefinedBy <> ;
  rdfs:label "Has Shape Tree Location"@en .

# ShapeTreeLocation class
#############################################################################
# A ShapeTreeLocation identifies a shape tree and the managed resource it is
# associated with, the focus node for shape validation, and the information
# needed to navigate the physical hierarchy in which that managed resource
# resides.
#############################################################################
:ShapeTreeLocation
  a rdfs:Class ;
  rdfs:comment "identifies a shape tree and the managed resource it is associated with, the focus node for shape validation, and the information needed to navigate the physical hierarchy in which that managed resource resides"@en ;
  rdfs:isDefinedBy <> ;
  rdfs:label "Shape Tree Location"@en .

:hasManagedResource
  a owl:ObjectProperty ;
  rdfs:domain :ShapeTreeLocation ;
  rdfs:comment "Identifies the managed resource associated with the shape tree location"@en ;
  rdfs:isDefinedBy <> ;
  rdfs:label "Has Managed Resource"@en .

:hasRootShapeTreeLocation
  a owl:ObjectProperty ;
  rdfs:range :ShapeTreeLocation ;
  rdfs:comment "Identifies the root shape tree location"@en ;
  rdfs:isDefinedBy <> ;
  rdfs:label "Has Root Shape Tree Location"@en .

:node
  a owl:ObjectProperty ;
  rdfs:domain :ShapeTreeLocation ;
  rdfs:comment "Identifies the focus node for shape validation in the associated managed resource"@en ;
  rdfs:isDefinedBy <> ;
  rdfs:label "Has Focus Node"@en .

:hasShapeTree
  a owl:ObjectProperty ;
  rdfs:range :ShapeTree ;
  rdfs:comment "Represents the IRI of a ShapeTree that is referenced by some subject"@en ;
  rdfs:isDefinedBy <> ;
  rdfs:label "Has ShapeTree Instance Root"@en .

################################################################
# Resource Type Shape Tree Definitions
################################################################

:NonRDFResourceTree
    a :ShapeTree ;
    :expectsType :NonRDFResource .

:ResourceTree
    a :ShapeTree ;
    :expectsType :Resource .

:ContainerTree
    a :ShapeTree ;
    :expectsType :NonRDFResource .
