@prefix rdf: <http://www.w3.org/1999/02/22-rdf-syntax-ns#> .
@prefix rdfs: <http://www.w3.org/2000/01/rdf-schema#> .
@prefix shex: <http://www.w3.org/ns/shex#> .
@prefix xsd: <http://www.w3.org/2001/XMLSchema#> .

# CSVM Ontology definition
shex: a owl:Ontology;
  dc:title "Shape Expression Vocabulary"@en;
  dc:description """This document describes the RDFS vocabulary description used in the Shape Expression Language (ShEx) [[shex-semantics]] along with the default JSON-LD Context and shape expression to validate RDF versions of shapes."""@en;
  dc:date "2017-04-12"^^xsd:date;
  dc:imports ;
  owl:versionInfo <https://github.com/shexSpec/shexspec.github.io/commit/07d3e76be478d8c7f8c2e9d3b1f95635890239e0>;
  rdfs:seeAlso <http://shex.io/shex-semantics>;
  .


# Class definitions
shex:Annotation a rdfs:Class;
  rdfs:label "Annotation"@en;
  rdfs:comment """Annotations provide a format-independent way to provide additional information about elements in a schema. """@en;
  rdfs:isDefinedBy shex: .
shex:EachOf a rdfs:Class;
  rdfs:label "Each Of"@en;
  rdfs:comment """A TripleExpression composed of one or more sub-expressions, all of which must match."""@en;
  rdfs:subClassOf shex:TripleExpression;
  rdfs:isDefinedBy shex: .
shex:IriStem a rdfs:Class;
  rdfs:label "IRI StemRange"@en;
  rdfs:comment """An IRI prefix (or wildcard) along with a set of excluded values, used for node matching."""@en;
  rdfs:subClassOf shex:StemRange;
  rdfs:isDefinedBy shex: .
shex:LanguageStem a rdfs:Class;
  rdfs:label "Language StemRange"@en;
  rdfs:comment """An Language prefix (or wildcard) along with a set of excluded values, used for node matching."""@en;
  rdfs:subClassOf shex:StemRange;
  rdfs:isDefinedBy shex: .
shex:LiteralStem a rdfs:Class;
  rdfs:label "Literal StemRange"@en;
  rdfs:comment """An Literal prefix (or wildcard) along with a set of excluded values, used for node matching."""@en;
  rdfs:subClassOf shex:StemRange;
  rdfs:isDefinedBy shex: .
shex:NodeConstraint a rdfs:Class;
  rdfs:label "Node Constraint"@en;
  rdfs:comment """A constraint on the type or value of an RDF Node."""@en;
  rdfs:subClassOf shex:ShapeExpression;
  rdfs:isDefinedBy shex: .
shex:NodeKind a rdfs:Class;
  rdfs:label "Node Kind"@en;
  rdfs:comment """The set of kinds of RDF Nodes."""@en;
  rdfs:isDefinedBy shex: .
shex:OneOf a rdfs:Class;
  rdfs:label "One Of"@en;
  rdfs:comment """A TripleExpression composed of one or more sub-expressions, one of which must match."""@en;
  rdfs:subClassOf shex:TripleExpression;
  rdfs:isDefinedBy shex: .
shex:Schema a rdfs:Class;
  rdfs:label "Schema"@en;
  rdfs:comment """A Schema contains the set of shapes, used for matching a focus node."""@en;
  rdfs:isDefinedBy shex: .
shex:SemAct a rdfs:Class;
  rdfs:label "Semantic Actions"@en;
  rdfs:comment """A list of Semantic Actions that serve as an extension point for Shape Expressions. They appear in lists in Schema's startActs and Shape, OneOf, EachOf and TripleConstraint's semActs."""@en;
  rdfs:isDefinedBy shex: .
shex:Shape a rdfs:Class;
  rdfs:label "Shape Or"@en;
  rdfs:comment """A shapes schema is captured in a Schema object where shapes is a mapping from shape label to shape expression."""@en;
  rdfs:subClassOf shex:ShapeExpression;
  rdfs:isDefinedBy shex: .
shex:ShapeAnd a rdfs:Class;
  rdfs:label "Shape And"@en;
  rdfs:comment """A ShapeExpression composed of one or more sub-expressions, all of which must match."""@en;
  rdfs:subClassOf shex:ShapeExpression;
  rdfs:isDefinedBy shex: .
shex:ShapeExpression a rdfs:Class;
  rdfs:label "Shape Expression"@en;
  rdfs:comment """The abstract class of Shape Expressions."""@en;
  rdfs:isDefinedBy shex: .
shex:ShapeExternal a rdfs:Class;
  rdfs:label "Shape External"@en;
  rdfs:comment """A reference to a shape defined in some external Schema."""@en;
  rdfs:subClassOf shex:ShapeExpression;
  rdfs:isDefinedBy shex: .
shex:ShapeNot a rdfs:Class;
  rdfs:label "Shape Not"@en;
  rdfs:comment """A ShapeNot is satisfied when it's included ShapeExpression is not satisfied."""@en;
  rdfs:subClassOf shex:ShapeExpression;
  rdfs:isDefinedBy shex: .
shex:ShapeOr a rdfs:Class;
  rdfs:label "Shape Or"@en;
  rdfs:comment """A ShapeExpression composed of one or more sub-expressions, one of which must match."""@en;
  rdfs:subClassOf shex:ShapeExpression;
  rdfs:isDefinedBy shex: .
shex:Stem a rdfs:Class;
  rdfs:label "Stem"@en;
  rdfs:comment """Abstract class for Stems"""@en;
  rdfs:isDefinedBy shex: .
shex:StemRange a rdfs:Class;
  rdfs:label "StemRange"@en;
  rdfs:comment """Abstract Class for Stem Ranges"""@en;
  rdfs:isDefinedBy shex: .
shex:TripleConstraint a rdfs:Class;
  rdfs:label "Triple Constraint"@en;
  rdfs:comment """A constraint on a triple having a specific predicate and optionally a shape expression used for matching values."""@en;
  rdfs:subClassOf shex:TripleExpression;
  rdfs:isDefinedBy shex: .
shex:TripleExpression a rdfs:Class;
  rdfs:label "Triple Expression"@en;
  rdfs:comment """The abstract class of Triple Expressions."""@en;
  rdfs:isDefinedBy shex: .
shex:Wildcard a rdfs:Class;
  rdfs:label "Wildcard"@en;
  rdfs:comment """Indicates that a stem is a Wildcard, rather than a URI prefix."""@en;
  rdfs:isDefinedBy shex: .

# Property definitions
shex:annotation a rdf:Property;
  rdfs:label "annotation"@en;
  rdfs:comment """Annotations on a TripleExpression."""@en;
  rdfs:domain [ owl:unionOf (shex:EachOf shex:OneOf shex:TripleConstraint)];
  rdfs:range shex:Annotation;
  rdfs:isDefinedBy shex: .
shex:closed a rdf:Property;
  rdfs:label "closed"@en;
  rdfs:comment """Indicates that a Shape is closed, meaning that it may contain no property values other than those used within TripleConstraints."""@en;
  rdfs:domain shex:Shape;
  rdfs:range xsd:boolean;
  rdfs:isDefinedBy shex: .
shex:code a rdf:Property;
  rdfs:label "code"@en;
  rdfs:comment """Code executed by Semantic Action."""@en;
  rdfs:domain shex:SemAct;
  rdfs:range xsd:string;
  rdfs:isDefinedBy shex: .
shex:datatype a rdf:Property;
  rdfs:label "datatype"@en;
  rdfs:comment """A datatype constraint."""@en;
  rdfs:domain shex:NodeConstraint;
  rdfs:range rdfs:Datatype;
  rdfs:isDefinedBy shex: .
shex:exclusion a rdf:Property;
  rdfs:label "exclusion"@en;
  rdfs:comment """Values that are excluded from value matching."""@en;
  rdfs:domain shex:StemRange;
  rdfs:range [ owl:unionOf (rdfs:Resource shex:Stem)];
  rdfs:isDefinedBy shex: .
shex:expression a rdf:Property;
  rdfs:label "expression"@en;
  rdfs:comment """Expression associated with the TripleExpression."""@en;
  rdfs:domain shex:Shape;
  rdfs:range shex:TripleExpression;
  rdfs:isDefinedBy shex: .
shex:expressions a rdf:Property;
  rdfs:label "expressions"@en;
  rdfs:comment """List of 2 or more expressions associated with the TripleExpression."""@en;
  rdfs:domain [ owl:unionOf (shex:EachOf shex:OneOf)];
  rdfs:range shex:TripleExpression;
  rdfs:isDefinedBy shex: .
shex:extra a rdf:Property;
  rdfs:label "extra"@en;
  rdfs:comment """Properties which may have extra values beyond those matched through a constraint."""@en;
  rdfs:domain shex:Shape;
  rdfs:range rdfs:Resource;
  rdfs:isDefinedBy shex: .
shex:flags a rdf:Property;
  rdfs:label "flags"@en;
  rdfs:comment """Regular expression flags"""@en;
  rdfs:domain shex:NodeConstraint;
  rdfs:range xsd:string;
  rdfs:isDefinedBy shex: .
shex:fractiondigits a rdf:Property;
  rdfs:label "fraction digits"@en;
  rdfs:comment """for "fractiondigits" constraints, v is less than or equals the number of digits to the right of the decimal place in the XML Schema canonical form[xmlschema-2] of the value of n, ignoring trailing zeros."""@en;
  rdfs:subPropertyOf shex:numericFacet;
  rdfs:domain shex:NodeConstraint;
  rdfs:range xsd:integer;
  rdfs:isDefinedBy shex: .
shex:inverse a rdf:Property;
  rdfs:label "inverse"@en;
  rdfs:comment """Constrains the subject of a triple, rather than the object."""@en;
  rdfs:domain shex:TripleConstraint;
  rdfs:range xsd:boolean;
  rdfs:isDefinedBy shex: .
shex:length a rdf:Property;
  rdfs:label "length"@en;
  rdfs:comment """The exact length of the value of the cell."""@en;
  rdfs:subPropertyOf shex:stringFacet;
  rdfs:domain shex:NodeConstraint;
  rdfs:range xsd:integer;
  rdfs:isDefinedBy shex: .
shex:max a rdf:Property;
  rdfs:label "maximum cardinality"@en;
  rdfs:comment """Maximum number of times this TripleExpression may match; -1 for "*""""@en;
  rdfs:domain [ owl:unionOf (shex:EachOf shex:OneOf shex:TripleConstraint)];
  rdfs:range xsd:integer;
  rdfs:isDefinedBy shex: .
shex:maxexclusive a rdf:Property;
  rdfs:label "max exclusive"@en;
  rdfs:comment """An atomic property that contains a single number that is the maximum valid value (exclusive)."""@en;
  rdfs:subPropertyOf shex:numericFacet;
  rdfs:domain shex:NodeConstraint;
  rdfs:range [ owl:unionOf (xsd:integer xsd:decimal xsd:double)];
  rdfs:isDefinedBy shex: .
shex:maxinclusive a rdf:Property;
  rdfs:label "max inclusive"@en;
  rdfs:comment """An atomic property that contains a single number that is the maximum valid value (inclusive)."""@en;
  rdfs:subPropertyOf shex:numericFacet;
  rdfs:domain shex:NodeConstraint;
  rdfs:range [ owl:unionOf (xsd:integer xsd:decimal xsd:double)];
  rdfs:isDefinedBy shex: .
shex:maxlength a rdf:Property;
  rdfs:label "max length"@en;
  rdfs:comment """A numeric atomic property that contains a single integer that is the maximum length of the value."""@en;
  rdfs:subPropertyOf shex:stringFacet;
  rdfs:domain shex:NodeConstraint;
  rdfs:range xsd:integer;
  rdfs:isDefinedBy shex: .
shex:min a rdf:Property;
  rdfs:label "minimum cardinatliy"@en;
  rdfs:comment """Minimum number of times this TripleExpression may match."""@en;
  rdfs:domain [ owl:unionOf (shex:EachOf shex:OneOf shex:TripleConstraint)];
  rdfs:range xsd:integer;
  rdfs:isDefinedBy shex: .
shex:minexclusive a rdf:Property;
  rdfs:label "min exclusive"@en;
  rdfs:comment """An atomic property that contains a single number that is the minimum valid value (exclusive)."""@en;
  rdfs:subPropertyOf shex:numericFacet;
  rdfs:domain shex:NodeConstraint;
  rdfs:range [ owl:unionOf (xsd:integer xsd:decimal xsd:double)];
  rdfs:isDefinedBy shex: .
shex:mininclusive a rdf:Property;
  rdfs:label "min inclusive"@en;
  rdfs:comment """An atomic property that contains a single number that is the minimum valid value (inclusive)."""@en;
  rdfs:subPropertyOf shex:numericFacet;
  rdfs:domain shex:NodeConstraint;
  rdfs:range [ owl:unionOf (xsd:integer xsd:decimal xsd:double)];
  rdfs:isDefinedBy shex: .
shex:minlength a rdf:Property;
  rdfs:label "min length"@en;
  rdfs:comment """An atomic property that contains a single integer that is the minimum length of the value."""@en;
  rdfs:subPropertyOf shex:stringFacet;
  rdfs:domain shex:NodeConstraint;
  rdfs:range xsd:integer;
  rdfs:isDefinedBy shex: .
shex:name a rdf:Property;
  rdfs:label "name"@en;
  rdfs:comment """Identifier of SemAct extension."""@en;
  rdfs:domain shex:SemAct;
  rdfs:range rdfs:Resource;
  rdfs:isDefinedBy shex: .
shex:nodeKind a rdf:Property;
  rdfs:label "node kind"@en;
  rdfs:comment """Restiction on the kind of node matched; restricted to the defined instances of NodeKind. One of shex:iri, shex:bnode, shex:literal, or shex:nonliteral."""@en;
  rdfs:domain shex:NodeConstraint;
  rdfs:range shex:NodeKind;
  rdfs:isDefinedBy shex: .
shex:numericFacet a rdf:Property;
  rdfs:label ""@en;
  rdfs:comment """Abstract property of numeric facets on a NodeConstraint."""@en;
  rdfs:subPropertyOf shex:xsFacet;
  rdfs:isDefinedBy shex: .
shex:object a rdf:Property;
  rdfs:label "object"@en;
  rdfs:comment """The object of an Annotation."""@en;
  rdfs:domain shex:Annotation;
  rdfs:range rdfs:Resource;
  rdfs:isDefinedBy shex: .
shex:pattern a rdf:Property;
  rdfs:label "pattern"@en;
  rdfs:comment """A regular expression used for matching a value."""@en;
  rdfs:subPropertyOf shex:stringFacet;
  rdfs:domain shex:NodeConstraint;
  rdfs:range xsd:string;
  rdfs:isDefinedBy shex: .
shex:predicate a rdf:Property;
  rdfs:label "predicate"@en;
  rdfs:comment """The predicate of a TripleConstraint or Annotation."""@en;
  rdfs:domain [ owl:unionOf (shex:Annotation shex:TripleConstraint)];
  rdfs:range rdfs:Resource;
  rdfs:isDefinedBy shex: .
shex:semActs a rdf:Property;
  rdfs:label "semantic action"@en;
  rdfs:comment """Semantic Actions on this TripleExpression."""@en;
  rdfs:domain [ owl:unionOf (shex:EachOf shex:OneOf shex:TripleConstraint)];
  rdfs:range shex:SemAct;
  rdfs:isDefinedBy shex: .
shex:shapeExpr a rdf:Property;
  rdfs:label "shape expression"@en;
  rdfs:comment """Shape Expression referenced by this shape."""@en;
  rdfs:domain shex:ShapeNot;
  rdfs:range shex:ShapeExpression;
  rdfs:isDefinedBy shex: .
shex:shapeExprs a rdf:Property;
  rdfs:label "shape expressions"@en;
  rdfs:comment """A list of 2 or more Shape Expressions referenced by this shape."""@en;
  rdfs:subPropertyOf shex:shapeExpr;
  rdfs:domain [ owl:unionOf (shex:ShapeAnd shex:ShapeOr)];
  rdfs:range shex:ShapeExpression;
  rdfs:isDefinedBy shex: .
shex:shapes a rdf:Property;
  rdfs:label "shapes"@en;
  rdfs:comment """Shapes in this Schema."""@en;
  rdfs:domain shex:Schema;
  rdfs:range shex:ShapeExpression;
  rdfs:isDefinedBy shex: .
shex:start a rdf:Property;
  rdfs:label "start"@en;
  rdfs:comment """A ShapeExpression matched against the focus node prior to any other mapped expressions."""@en;
  rdfs:domain shex:Schema;
  rdfs:range shex:ShapeExpression;
  rdfs:isDefinedBy shex: .
shex:startActs a rdf:Property;
  rdfs:label "start actions"@en;
  rdfs:comment """Semantic Actions run on the Schema."""@en;
  rdfs:domain shex:Schema;
  rdfs:range shex:SemAct;
  rdfs:isDefinedBy shex: .
shex:stem a rdf:Property;
  rdfs:label "stem"@en;
  rdfs:comment """A stem value used for matching or excluding values."""@en;
  rdfs:domain [ owl:unionOf (shex:Stem shex:StemRange)];
  rdfs:range [ owl:unionOf (xsd:anyUri shex:Wildcard)];
  rdfs:isDefinedBy shex: .
shex:stringFacet a rdf:Property;
  rdfs:label ""@en;
  rdfs:comment """An abstract property of string facets on a NodeConstraint."""@en;
  rdfs:subPropertyOf shex:xsFacet;
  rdfs:isDefinedBy shex: .
shex:totaldigits a rdf:Property;
  rdfs:label "total digits"@en;
  rdfs:comment """for "totaldigits" constraints, v equals the number of digits in the XML Schema canonical form[xmlschema-2] of the value of n"""@en;
  rdfs:subPropertyOf shex:numericFacet;
  rdfs:domain shex:NodeConstraint;
  rdfs:range xsd:integer;
  rdfs:isDefinedBy shex: .
shex:valueExpr a rdf:Property;
  rdfs:label "value expression"@en;
  rdfs:comment """A ShapeExpression used for matching the object (or subject if inverted) of a TripleConstraint."""@en;
  rdfs:domain shex:TripleConstraint;
  rdfs:range shex:ShapeExpression;
  rdfs:isDefinedBy shex: .
shex:values a rdf:Property;
  rdfs:label "values"@en;
  rdfs:comment """A value restriction on a NodeConstraint."""@en;
  rdfs:domain shex:NodeConstraint;
  rdfs:range [ owl:unionOf (rdfs:Resource shex:Stem shex:StemRange)];
  rdfs:isDefinedBy shex: .
shex:xsFacet a rdf:Property;
  rdfs:label ""@en;
  rdfs:comment """An abstract property of string and numeric facets on a NodeConstraint."""@en;
  rdfs:domain shex:NodeConstraint;
  rdfs:isDefinedBy shex: .

# Datatype definitions

# Instance definitions
shex:bnode a shex:NodeKind;
  rdfs:label "bnode"@en;
  rdfs:comment """Requires node to be a Blank Node"""@en;
  rdfs:isDefinedBy shex: .
shex:iri a shex:NodeKind;
  rdfs:label "iri"@en;
  rdfs:comment """Requires node to be an IRI"""@en;
  rdfs:isDefinedBy shex: .
shex:literal a shex:NodeKind;
  rdfs:label "literal"@en;
  rdfs:comment """Requires node to be an rdf:Literal"""@en;
  rdfs:isDefinedBy shex: .
shex:nonliteral a shex:NodeKind;
  rdfs:label "nonliteral"@en;
  rdfs:comment """Requires node to be a Blank Node or IRI"""@en;
  rdfs:isDefinedBy shex: .
